completness proof

theories/symbolic.v
@@ -5,52 +5,52 @@ Import ListNotations.
 
 (** Symbolic expressions *)
 Inductive sym_expr :=
-    | Sbool (b: bool)
-    | Sint (i: Z)
-    | Svar (s : string)
-    | Sop (o : op) (e1 e2 : sym_expr)
-    | Sclo (t: term) (sigma: var -> sym_expr).
+  | Sbool (b: bool)
+  | Sint (i: Z)
+  | Svar (s : string)
+  | Sop (o : op) (e1 e2 : sym_expr)
+  | Sclo (t: term) (sigma: var -> sym_expr).
 
 Inductive sym_result :=
-    | SRexpr (e : sym_expr)
-    | SRempty
-    | SRconflict.
+  | SRexpr (e : sym_expr)
+  | SRempty
+  | SRconflict.
 
 Fixpoint eval_sym_expr (e : sym_expr) (env : string -> value) : value :=
-    match e with
-    | Sbool b => Bool b
-    | Sint i => Int i
-    | Svar s => env s
-    | Sop Add e1 e2 =>
-        match eval_sym_expr e1 env, eval_sym_expr e2 env with
-        | Int i1, Int i2 => Int (i1 + i2)%Z
-        | _, _ => Int 0%Z (* unreachable *)
-        end
-    | Sop Eq e1 e2 =>
-        match eval_sym_expr e1 env, eval_sym_expr e2 env with
-        | Int i1, Int i2 => Bool (i1 =? i2)%Z
-        | _, _ => Bool false (* unreachable *)
-        end
-    | Sclo t s => Closure t (fun x => eval_sym_expr (s x) env)
-    end.
+  match e with
+  | Sbool b => Bool b
+  | Sint i => Int i
+  | Svar s => env s
+  | Sop Add e1 e2 =>
+      match eval_sym_expr e1 env, eval_sym_expr e2 env with
+      | Int i1, Int i2 => Int (i1 + i2)%Z
+      | _, _ => Int 0%Z (* unreachable *)
+      end
+  | Sop Eq e1 e2 =>
+      match eval_sym_expr e1 env, eval_sym_expr e2 env with
+      | Int i1, Int i2 => Bool (i1 =? i2)%Z
+      | _, _ => Bool false (* unreachable *)
+      end
+  | Sclo t s => Closure t (fun x => eval_sym_expr (s x) env)
+  end.
 
 (** Symbolic continuations *)
 Inductive sym_cont :=
-    | SCAppL (t1 : term) (* [ t1 \square ] *)
-    | SCAppR (t2 : term) (* [ \square t2 ] *)
-    | SCClosure (t_cl: {bind term}) (sigma_cl: var -> sym_expr)
-    | SCDefault (o : option sym_expr) (ts: list term) (tj: term) (tc: term)
-    | SCDefaultBase (tc: term)
-    .
+  | SCAppL (t1 : term) (* [ t1 \square ] *)
+  | SCAppR (t2 : term) (* [ \square t2 ] *)
+  | SCClosure (t_cl: {bind term}) (sigma_cl: var -> sym_expr)
+  | SCDefault (o : option sym_expr) (ts: list term) (tj: term) (tc: term)
+  | SCDefaultBase (tc: term)
+  .
 
 (** Symbolic constraints *)
 Inductive sym_constraint :=
-    | Eq (e1 e2 : sym_expr)
-    | IsTrue (e : sym_expr)
-    | And (c1 c2 : sym_constraint)
-    | Or (c1 c2 : sym_constraint)
-    | Not (c : sym_constraint)
-    .
+  | Eq (e1 e2 : sym_expr)
+  | IsTrue (e : sym_expr)
+  | And (c1 c2 : sym_constraint)
+  | Or (c1 c2 : sym_constraint)
+  | Not (c : sym_constraint)
+  .
 
 (** Symbolic paths *)
 Definition sym_path := list sym_constraint.
@@ -59,146 +59,147 @@ Definition sym_path := list sym_constraint.
 Definition sym_store := var -> sym_expr.
 
 Fixpoint eval_sym_constraint (env : string -> value) (c : sym_constraint) :=
-    match c with
-    | Eq e1 e2 => value_eqb (eval_sym_expr e1 env) (eval_sym_expr e1 env)
-    | IsTrue e =>
-        match eval_sym_expr e env with
-        | Bool b => b
-        | _ => false
-        end
-    | And c1 c2 =>
-        (eval_sym_constraint env c1 && eval_sym_constraint env c2)%bool
-    | Or c1 c2 =>
-        (eval_sym_constraint env c1 || eval_sym_constraint env c2)%bool
-    | Not c =>
-        negb (eval_sym_constraint env c)
-    end.
+  match c with
+  | Eq e1 e2 => value_eqb (eval_sym_expr e1 env) (eval_sym_expr e1 env)
+  | IsTrue e =>
+      match eval_sym_expr e env with
+      | Bool b => b
+      | _ => false
+      end
+  | And c1 c2 =>
+      (eval_sym_constraint env c1 && eval_sym_constraint env c2)%bool
+  | Or c1 c2 =>
+      (eval_sym_constraint env c1 || eval_sym_constraint env c2)%bool
+  | Not c =>
+      negb (eval_sym_constraint env c)
+  end.
 
 Definition eval_sym_path (env : string -> value) (p : sym_path) :=
-    forallb (eval_sym_constraint env) p.
+  forallb (eval_sym_constraint env) p.
 
 (** Symbolic states *)
 Inductive sym_state :=
-    (* Symbolic evaluation mode *)
-    | sym_mode_eval (e : term) (stack : list sym_cont) (path : sym_path) (env : sym_store)
-    (* Symbolic continuation mode *)
-    | sym_mode_cont (stack : list sym_cont) (path : sym_path) (env : sym_store) (r : sym_result).
+  (* Symbolic evaluation mode *)
+  | sym_mode_eval (e : term) (stack : list sym_cont) (path : sym_path) (env : sym_store)
+  (* Symbolic continuation mode *)
+  | sym_mode_cont (stack : list sym_cont) (path : sym_path) (env : sym_store) (r : sym_result).
 
 
 Inductive sym_cred: sym_state -> sym_state -> Prop :=
-    | sym_cred_var:
-        forall x kappa phi sigma,
-        sym_cred
-            (sym_mode_eval (Var x) kappa phi sigma)
-            (sym_mode_cont kappa phi sigma (SRexpr (sigma x)))
+  | sym_cred_var:
+      forall x kappa phi sigma,
+      sym_cred
+          (sym_mode_eval (Var x) kappa phi sigma)
+          (sym_mode_cont kappa phi sigma (SRexpr (sigma x)))
 
-    | sym_cred_app:
-        forall t1 t2 kappa phi sigma,
-        sym_cred
-            (sym_mode_eval (App t1 t2) kappa phi sigma)
-            (sym_mode_eval t1 ((SCAppR t2) :: kappa) phi sigma)
-    
-    | sym_cred_clo:
-        forall t kappa phi sigma,
-        sym_cred
-            (sym_mode_eval (Lam t) kappa phi sigma)
-            (sym_mode_cont kappa phi sigma (SRexpr (Sclo t sigma)))
+  | sym_cred_app:
+      forall t1 t2 kappa phi sigma,
+      sym_cred
+          (sym_mode_eval (App t1 t2) kappa phi sigma)
+          (sym_mode_eval t1 ((SCAppR t2) :: kappa) phi sigma)
+  
+  | sym_cred_clo:
+      forall t kappa phi sigma,
+      sym_cred
+          (sym_mode_eval (Lam t) kappa phi sigma)
+          (sym_mode_cont kappa phi sigma (SRexpr (Sclo t sigma)))
 
-    | sym_cred_arg:
-        forall t2 kappa phi sigma tcl sigmacl,
-        sym_cred
-            (sym_mode_cont ((SCAppR t2)::kappa) phi sigma (SRexpr (Sclo tcl sigmacl)))
-            (sym_mode_eval t2 ((SCClosure tcl sigmacl)::kappa) phi sigma)
+  | sym_cred_arg:
+      forall t2 kappa phi sigma tcl sigmacl,
+      sym_cred
+          (sym_mode_cont ((SCAppR t2)::kappa) phi sigma (SRexpr (Sclo tcl sigmacl)))
+          (sym_mode_eval t2 ((SCClosure tcl sigmacl)::kappa) phi sigma)
 
-    | sym_cred_beta:
-        forall tcl sigmacl kappa phi sigma v,
-        sym_cred
-            (sym_mode_cont ((SCClosure tcl sigmacl)::kappa) phi sigma (SRexpr v))
-            (sym_mode_eval tcl kappa phi (v .: sigmacl))
+  | sym_cred_beta:
+      forall tcl sigmacl kappa phi sigma v,
+      sym_cred
+          (sym_mode_cont ((SCClosure tcl sigmacl)::kappa) phi sigma (SRexpr v))
+          (sym_mode_eval tcl kappa phi (v .: sigmacl))
 
 
-    | sym_cred_default:
-        forall ts tj tc kappa phi sigma,
-        sym_cred
-            (sym_mode_eval (Default ts tj tc) kappa phi sigma)
-            (sym_mode_cont ((SCDefault None ts tj tc)::kappa) phi sigma SRempty)
+  | sym_cred_default:
+      forall ts tj tc kappa phi sigma,
+      sym_cred
+          (sym_mode_eval (Default ts tj tc) kappa phi sigma)
+          (sym_mode_cont ((SCDefault None ts tj tc)::kappa) phi sigma SRempty)
 
-    | sym_cred_defaultunpack:
-        forall o th ts tj tc kappa phi sigma,
-        sym_cred
-            (sym_mode_cont ((SCDefault o (th::ts) tj tc)::kappa) phi sigma SRempty)
-            (sym_mode_eval th ((SCDefault o ts tj tc)::kappa) phi sigma)
+  | sym_cred_defaultunpack:
+      forall o th ts tj tc kappa phi sigma,
+      sym_cred
+          (sym_mode_cont ((SCDefault o (th::ts) tj tc)::kappa) phi sigma SRempty)
+          (sym_mode_eval th ((SCDefault o ts tj tc)::kappa) phi sigma)
 
-    | sym_cred_defaultnone:
-        forall ts tj tc kappa phi sigma v,
-        sym_cred
-            (sym_mode_cont ((SCDefault None ts tj tc)::kappa) phi sigma (SRexpr v))
-            (sym_mode_cont ((SCDefault (Some v) ts tj tc)::kappa) phi sigma SRempty)
+  | sym_cred_defaultnone:
+      forall ts tj tc kappa phi sigma v,
+      sym_cred
+          (sym_mode_cont ((SCDefault None ts tj tc)::kappa) phi sigma (SRexpr v))
+          (sym_mode_cont ((SCDefault (Some v) ts tj tc)::kappa) phi sigma SRempty)
 
-    | sym_cred_defaultconflict:
-        forall ts tj tc kappa phi sigma v v',
-        sym_cred
-            (sym_mode_cont ((SCDefault (Some v) ts tj tc)::kappa) phi sigma (SRexpr v'))
-            (sym_mode_cont kappa phi sigma SRconflict)
+  | sym_cred_defaultconflict:
+      forall ts tj tc kappa phi sigma v v',
+      sym_cred
+          (sym_mode_cont ((SCDefault (Some v) ts tj tc)::kappa) phi sigma (SRexpr v'))
+          (sym_mode_cont kappa phi sigma SRconflict)
 
-    | sym_cred_defaultvalue:
-        forall v tj tc kappa phi sigma,
-        sym_cred
-            (sym_mode_cont ((SCDefault (Some v) [] tj tc)::kappa) phi sigma SRempty)
-            (sym_mode_cont kappa phi sigma (SRexpr v))
+  | sym_cred_defaultvalue:
+      forall v tj tc kappa phi sigma,
+      sym_cred
+          (sym_mode_cont ((SCDefault (Some v) [] tj tc)::kappa) phi sigma SRempty)
+          (sym_mode_cont kappa phi sigma (SRexpr v))
 
-    (* | cred_defaultnonefinal: (* not needed *)
-        (* $\lcont \mathtt{Def}(\synnone, [], e_j, e_c) \cons \kappa, \sigma, v \rcont \leadsto \lcont \kappa, \sigma, v \rcont$ \hfill $v \neq \synempty, \synconflict$ *)
-        todo *)
+  (* | cred_defaultnonefinal: (* not needed *)
+      (* $\lcont \mathtt{Def}(\synnone, [], e_j, e_c) \cons \kappa, \sigma, v \rcont \leadsto \lcont \kappa, \sigma, v \rcont$ \hfill $v \neq \synempty, \synconflict$ *)
+      todo *)
 
-    | sym_cred_defaultbase:
-        forall tj tc kappa phi sigma,
-        sym_cred
-            (sym_mode_cont ((SCDefault None [] tj tc)::kappa) phi sigma SRempty)
-            (sym_mode_eval tj ((SCDefaultBase tc)::kappa) phi sigma)
+  | sym_cred_defaultbase:
+      forall tj tc kappa phi sigma,
+      sym_cred
+          (sym_mode_cont ((SCDefault None [] tj tc)::kappa) phi sigma SRempty)
+          (sym_mode_eval tj ((SCDefaultBase tc)::kappa) phi sigma)
 
-    | sym_cred_defaultbasetrue:
-        forall tc kappa phi sigma v,
-        sym_cred
-            (sym_mode_cont ((SCDefaultBase tc)::kappa) phi sigma (SRexpr v))
-            (sym_mode_eval tc kappa (IsTrue v :: phi) sigma)
+  | sym_cred_defaultbasetrue:
+      forall tc kappa phi sigma v,
+      sym_cred
+          (sym_mode_cont ((SCDefaultBase tc)::kappa) phi sigma (SRexpr v))
+          (sym_mode_eval tc kappa (IsTrue v :: phi) sigma)
 
-    | sym_cred_defaultbasefalse:
-        forall tc kappa phi sigma v,
-        sym_cred
-            (sym_mode_cont ((SCDefaultBase tc)::kappa) phi sigma (SRexpr v))
-            (sym_mode_cont kappa (Not (IsTrue v) :: phi) sigma SRempty)
+  | sym_cred_defaultbasefalse:
+      forall tc kappa phi sigma v,
+      sym_cred
+          (sym_mode_cont ((SCDefaultBase tc)::kappa) phi sigma (SRexpr v))
+          (sym_mode_cont kappa (Not (IsTrue v) :: phi) sigma SRempty)
 
-    | sym_cred_empty:
-        forall k kappa phi sigma,
-        (forall o ts tj tc, k <> SCDefault o ts tj tc) ->
-        sym_cred
-            (sym_mode_cont (k::kappa) phi sigma SRempty)
-            (sym_mode_cont kappa phi sigma SRempty)
+  | sym_cred_empty:
+      forall k kappa phi sigma,
+      (forall o ts tj tc, k <> SCDefault o ts tj tc) ->
+      sym_cred
+          (sym_mode_cont (k::kappa) phi sigma SRempty)
+          (sym_mode_cont kappa phi sigma SRempty)
 
-    | sym_cred_conflict:
-        forall k kappa phi sigma,
-        sym_cred
-            (sym_mode_cont (k::kappa) phi sigma SRconflict)
-            (sym_mode_cont kappa phi sigma SRconflict)
+  | sym_cred_conflict:
+      forall k kappa phi sigma,
+      sym_cred
+          (sym_mode_cont (k::kappa) phi sigma SRconflict)
+          (sym_mode_cont kappa phi sigma SRconflict)
 
-    | sym_cred_confict_intro:
-        forall kappa phi sigma,
-        sym_cred
-            (sym_mode_eval Conflict kappa phi sigma)
-            (sym_mode_cont kappa phi sigma SRconflict)
+  | sym_cred_confict_intro:
+      forall kappa phi sigma,
+      sym_cred
+          (sym_mode_eval Conflict kappa phi sigma)
+          (sym_mode_cont kappa phi sigma SRconflict)
 
-    | sym_cred_empty_intro:
-        forall kappa phi sigma,
-        sym_cred
-            (sym_mode_eval Empty kappa phi sigma)
-            (sym_mode_cont kappa phi sigma SRempty)
-    .
+  | sym_cred_empty_intro:
+      forall kappa phi sigma,
+      sym_cred
+          (sym_mode_eval Empty kappa phi sigma)
+          (sym_mode_cont kappa phi sigma SRempty)
+  .
 
 (**
     What it means for a concrete and a symbolic value
     to be related with respect to an assignement of free variables
 *)
+
 Definition similar_value (env : string -> value) (v : value) (sym_v : sym_expr) :=
     v = eval_sym_expr sym_v env.
 
@@ -277,47 +278,120 @@ Proof.
     induction e; try easy; simpl in *.
     - eexists. *)
 
+Definition no_closure (env : string -> value) :=
+    forall x tcl sigmacl, env x = Closure tcl sigmacl -> False.
+
+Theorem boring_lemma:
+  forall env sigma sym_sigma v sym_v,
+    similar_value env v sym_v ->
+    similar_env env sigma sym_sigma ->
+    similar_env env (v .: sigma) (sym_v .: sym_sigma).
+Proof.
+  intros * Hsim_v Hsim_env x.
+  unfold similar_value in *; subst.
+  destruct x; simpl; try easy.
+  apply Hsim_env.
+Qed.
+
 (**
     Every concrete transition can be simulated
     by a symbolic one
 *)
 Theorem sym_cred_complete:
-    forall env s1 s2 sym_s1,
-        similar env s1 sym_s1 ->
-        cred s1 s2 ->
-        exists sym_s2,
-            similar env s2 sym_s2 /\ sym_cred sym_s1 sym_s2.
+  forall env s1 s2 sym_s1,
+    no_closure env ->
+    similar env s1 sym_s1 ->
+    cred s1 s2 ->
+    exists sym_s2,
+      similar env s2 sym_s2 /\ sym_cred sym_s1 sym_s2.
 Proof.
-    intros * Hsim1 Hred.
-    induction Hred.
-    - inversion Hsim1; subst.
-        now repeat econstructor.
-    - inversion Hsim1; subst.
-        now repeat econstructor.
-    - inversion Hsim1; subst.
-        repeat econstructor; eauto.
-        unfold similar_value. simpl.
-        f_equal. now apply functional_extensionality.
-    - inversion Hsim1; subst.
-        inversion H2; subst.
-        inversion H5; subst.
-        inversion H1; subst.
-        inversion H0; subst.
-        (* AAHA we have a problem if some free vars evaluate to closures *)
-        admit.
-    - inversion Hsim1; subst.
-        admit.
-    - inversion Hsim1; subst.
-        admit.
-    - admit.
-    - admit.
-    - admit.
-    - admit.
-    - admit.
-    - admit.
-    - admit.
-    - admit.
-    - admit.
-    - admit.
-    - admit.
-Admitted.
+  intros * Hclo Hsim1 Hred.
+  induction Hred.
+  - inversion Hsim1; subst.
+    now repeat econstructor.
+  - inversion Hsim1; subst.
+    now repeat econstructor.
+  - inversion Hsim1; subst.
+    repeat econstructor; eauto.
+    unfold similar_value. simpl.
+    f_equal. now apply functional_extensionality.
+  - inversion Hsim1; subst.
+    inversion H2; subst.
+    inversion H5; subst.
+    inversion H1; subst.
+    inversion H0; subst.
+    destruct sym_v; try easy.
+    + simpl in H4. exfalso. eapply Hclo; eauto.
+    + simpl in H4. destruct o; try easy.
+      destruct (eval_sym_expr sym_v1); try easy.
+      destruct (eval_sym_expr sym_v2); try easy.
+      destruct (eval_sym_expr sym_v1); try easy.
+      destruct (eval_sym_expr sym_v2); try easy.
+    + simpl in H4. injection H4 as -> ->.
+      repeat econstructor; eauto.
+  - inversion Hsim1; subst.
+    inversion H5; subst.
+    inversion H2; subst.
+    inversion H4; subst.
+    repeat econstructor; eauto.
+    now apply boring_lemma.
+  - inversion Hsim1; subst.
+    now repeat econstructor.
+  - inversion Hsim1; subst.
+    inversion H2; subst.
+    inversion H5; subst.
+    inversion H1; subst.
+    + now repeat econstructor.
+    + now repeat econstructor.
+  - inversion Hsim1; subst.
+    inversion H2; subst.
+    inversion H1; subst.
+    inversion H5; subst.
+    now repeat econstructor.
+  - inversion Hsim1; subst.
+    inversion H2; subst.
+    inversion H1; subst.
+    inversion H5; subst.
+    now repeat econstructor.
+  - inversion Hsim1; subst.
+    inversion H2; subst.
+    inversion H1; subst.
+    inversion H5; subst.
+    now repeat econstructor.
+  - inversion Hsim1; subst.
+    inversion H2; subst.
+    inversion H1; subst.
+    inversion H5; subst.
+    now repeat econstructor.
+  - inversion Hsim1; subst.
+    inversion H2; subst.
+    inversion H1; subst.
+    inversion H5; subst.
+    inversion H0.
+    repeat econstructor; eauto.
+    simpl. now rewrite <- H4.
+  - inversion Hsim1; subst.
+    inversion H2; subst.
+    inversion H1; subst.
+    inversion H5; subst.
+    inversion H0.
+    repeat econstructor; eauto.
+    simpl. now rewrite <- H4.
+  - inversion Hsim1; subst.
+    inversion H6; subst.
+    inversion H3; subst.
+    repeat econstructor; auto.
+    inversion H2; subst; try easy.
+    + intros * [=<-<-<-<-].
+      now eapply H.
+    + intros * [=<-<-<-<-].
+      now eapply H.
+  - inversion Hsim1; subst.
+    inversion H2; subst.
+    inversion H5; subst.
+    now repeat econstructor.
+  - inversion Hsim1; subst.
+    now repeat econstructor.
+  - inversion Hsim1; subst.
+    now repeat econstructor.
+Qed.
